code/blake2b/Hacl.Impl.Blake2b.Partial2.fst
@@ -1,0 +1,130 @@
+module Hacl.Impl.Blake2b.Partial2
+
+open FStar.Mul
+open FStar.HyperStack
+open FStar.HyperStack.ST
+
+open Lib.IntTypes
+open Lib.Buffer
+open Lib.ByteBuffer
+open Lib.LoopCombinators
+
+open Hacl.Impl.Blake2b
+
+module ST = FStar.HyperStack.ST
+module Seq = Lib.Sequence
+module Loops = Lib.LoopCombinators
+module Spec = Spec.Blake2
+
+#set-options "--z3rlimit 50 --max_ifuel 0 --max_fuel 0"
+
+
+assume val to_size128: nat -> Tot size128_t
+
+
+val declassify_word: word_t -> Tot (Spec.pub_word_t Spec.Blake2.Blake2B)
+let declassify_word x =
+  let px = Lib.RawIntTypes.u64_to_UInt64 x in
+  let l :uint_t (Spec.wt Spec.Blake2.Blake2B) PUB = px in
+  l
+
+
+val declassify_word_to_size: word_t -> Tot size_t
+let declassify_word_to_size x =
+  let x32 = to_u32 x in
+  let y32 = Lib.RawIntTypes.u32_to_UInt32 x32 in
+  let l :size_t = Lib.RawIntTypes.size_from_UInt32 y32 in
+  l
+
+
+
+(** Define the state *)
+noeq type state_r = {
+  hash: hash_wp;
+  prev: p:size128_t{v p <= Spec.Blake2.max_limb Spec.Blake2B};
+  kk: size_t;
+  nblock: size_t;
+  pl: l:size_t{v l <= v size_block};
+  block: block_p;
+}
+
+
+type state_inv (h:mem) (s:state_r) =
+  live h s.hash /\ live h s.block /\ disjoint s.hash s.block
+
+
+val blake2b_init_partial:
+    state: state_r
+  -> kk: size_t{v kk <= 64}
+  -> k: lbuffer uint8 kk
+  -> nn: size_t{1 <= v nn /\ v nn <= 64} ->
+  Stack state_r
+  (requires fun h ->
+    live h state.hash /\ live h k /\
+    disjoint state.hash k)
+  (ensures  fun h0 _ h1 ->
+    modifies1 state.hash h0 h1)
+
+let blake2b_init_partial state kk k nn =
+  blake2b_init state.hash kk k nn;
+  [@inline_let]
+  let prev = if kk =. 0ul then 0 else 128 in
+  { state with
+    prev = to_size128 prev;
+    kk = kk;
+    nblock = 0ul;}
+
+
+
+inline_for_extraction
+val blake2b_update_partial:
+    state:state_r
+  -> ll:size_t
+  -> input:lbuffer uint8 ll ->
+  Stack state_r
+  (requires fun h ->
+    state_inv h state /\ live h input /\
+    disjoint state.hash input /\ disjoint state.block input /\
+    v state.kk <= 64 /\ (if v state.kk = 0 then v ll < pow2 128 else v ll + 128 < pow2 128))
+  (ensures  fun h0 _ h1 ->
+    modifies2 state.hash state.block h0 h1)
+
+let blake2b_update_partial state ll input =
+  let n = ll /. size_block in
+  let r = ll %. size_block in
+  let h0 = ST.get () in
+  loop_nospec #h0 n state.hash
+  (fun i ->
+    let block = sub input (i *. size_block) size_block in
+    let h1 = ST.get () in
+    blake2b_update_block state.hash (secret state.prev) block);
+  (* Compute the remaining space in the partial block *)
+  let rem: r:size_t{v r <= v size_block} = size_block -. state.pl in
+  (* Copy all input or the size available in the partial block *)
+  let ll0 = if r <=. rem then ll else rem in
+  let input0 = sub input 0ul ll0 in
+  update_sub #MUT #uint8 #size_block state.block state.pl ll0 input0;
+  if not (ll0 =. rem) then state // This needs to be updated
+  else (
+    blake2b_update_block state.hash (secret state.prev) state.block;
+    state // This needs to be updated
+  )
+
+
+
+val blake2b_finish_partial:
+    nn:size_t{1 <= v nn /\ v nn <= 64}
+  -> output:lbuffer uint8 nn
+  -> state:state_r ->
+  Stack unit
+    (requires fun h ->
+      state_inv h state /\ live h output
+      /\ disjoint output state.hash)
+    (ensures  fun h0 _ h1 ->
+      modifies1 output h0 h1 /\
+      h1.[|output|] == Spec.Blake2.blake2_finish Spec.Blake2B h0.[|state.hash|] (v nn))
+
+let blake2b_finish_partial nn output state =
+  let empty = create 0ul (u8 0) in
+  blake2b_update_last state.hash state.prev 0ul empty;
+  blake2b_finish nn output state.hash
